KZG_BatchOpening_knowledge_soundness.thy
@@ -1,0 +1,663 @@
+theory KZG_BatchOpening_knowledge_soundness
+
+imports KZG_BatchOpening_binding
+begin
+
+(*TODOD change discrp*)
+text \<open>We show knowledge soundness oriented at the definition in the PLONK paper (see section 3.1
+in the PLONK paper: https://eprint.iacr.org/2019/953.pdf). However, we show the property only for 
+a commitment to one polynomial to stay consistent with the other proofs in this work. Due to the 
+layout of the property though, this proof should be easily extendable to multiple polynomials 
+and thus serve as a strong basis for a proof for the full PLONK version.\<close>
+
+locale knowledge_sound_game_def = bind_game_proof
+begin
+
+type_synonym 'e' calc_vector = "'e' mod_ring list"
+
+type_synonym ('a', 'e')  adversary_1 = 
+  "'a' pk \<Rightarrow> 
+ ('a' commit \<times> 'e' calc_vector) spmf"
+
+type_synonym ('a', 'e')  adversary_2 = 
+  "'a' pk \<Rightarrow> 'a' commit \<Rightarrow> 'e' calc_vector \<Rightarrow> 
+   ('e' eval_position \<times> 'e' eval_position set\<times> 'e' polynomial \<times> 'a' eval_witness) spmf"
+
+type_synonym ('a', 'e') extractor = 
+  "'a' commit \<Rightarrow> 'e' calc_vector \<Rightarrow> 
+    'e' mod_ring poly"
+
+definition knowledge_soundness_game :: "('a, 'e) extractor \<Rightarrow> ('a, 'e) adversary_1 \<Rightarrow> ('a, 'e) adversary_2 
+  \<Rightarrow> bool spmf"
+  where "knowledge_soundness_game E \<A> \<A>' = TRY do {
+  PK \<leftarrow> key_gen;
+  (C,calc_vec) \<leftarrow> \<A> PK;
+  _ :: unit \<leftarrow> assert_spmf (length PK = length calc_vec 
+                          \<and> C = fold (\<lambda> i acc. acc \<otimes>\<^bsub>G\<^sub>p\<^esub> PK!i ^\<^bsub>G\<^sub>p\<^esub> (calc_vec!i)) [0..<length PK] \<one>\<^bsub>G\<^sub>p\<^esub>);  
+  let \<phi> = E C calc_vec;
+  (i, B, r_x, w_B) \<leftarrow> \<A>' PK C calc_vec;
+  _ ::unit \<leftarrow> assert_spmf (i \<in> B  \<and> valid_batch_msg r_x w_B B);
+  return_spmf (VerifyEvalBatch PK C B r_x w_B \<and> poly r_x i \<noteq> poly \<phi> i)} ELSE return_spmf False"
+
+definition knowledge_soundness_game_advantage :: "('a, 'e) extractor \<Rightarrow> ('a, 'e) adversary_1 \<Rightarrow> ('a, 'e) adversary_2 
+   \<Rightarrow> real"
+  where "knowledge_soundness_game_advantage E \<A> \<A>' \<equiv> spmf (knowledge_soundness_game E \<A> \<A>') True"
+
+subsubsection \<open>reduction definition\<close>
+
+definition knowledge_soundness_reduction
+  :: "('a, 'e) extractor \<Rightarrow> ('a, 'e) adversary_1 \<Rightarrow> ('a, 'e) adversary_2 \<Rightarrow> ('a, 'e) adversary"                     
+where
+  "knowledge_soundness_reduction E \<A> \<A>' PK = do {
+  (C,calc_vec) \<leftarrow> \<A> PK;
+  _ :: unit \<leftarrow> assert_spmf (length PK = length calc_vec 
+                          \<and> C = fold (\<lambda> i acc. acc \<otimes>\<^bsub>G\<^sub>p\<^esub> PK!i ^\<^bsub>G\<^sub>p\<^esub> (calc_vec!i)) [0..<length PK] \<one>\<^bsub>G\<^sub>p\<^esub>);  
+  let \<phi> = E C calc_vec;
+  (i, B, r_x, w_B) \<leftarrow> \<A>' PK C calc_vec;
+  let \<phi>_i = poly \<phi> i;
+  let w_i = createWitness PK \<phi> i;
+  return_spmf (C, i, \<phi>_i, w_i, B, w_B, r_x)}"
+
+subsubsection \<open>Extractor definition\<close>
+fun E :: "('a, 'e) extractor" where 
+  "E C calc_vec = Poly calc_vec"
+
+subsubsection \<open>alternative definitions for easier proving + their equivalence proofs\<close>
+
+lemma pull_down_assert_spmf_with_return:
+"do {
+    z::'z \<leftarrow> Z:: 'z spmf;
+    x::'x \<leftarrow> (X:: 'z \<Rightarrow> 'x spmf) z;
+    _ :: unit \<leftarrow> assert_spmf((f::'z \<Rightarrow> 'x \<Rightarrow> bool) z x);
+    y::'y \<leftarrow> (Y:: 'z \<Rightarrow> 'x \<Rightarrow> 'y spmf) z x;
+    _ :: unit \<leftarrow> assert_spmf ((A::'y \<Rightarrow> bool) y);
+    return_spmf ((g::'z \<Rightarrow> 'x \<Rightarrow> 'y \<Rightarrow> bool) z x y) }
+  = do {
+    z::'z \<leftarrow> Z:: 'z spmf;
+    x::'x \<leftarrow> (X:: 'z \<Rightarrow> 'x spmf) z;
+    y::'y \<leftarrow> (Y:: 'z \<Rightarrow> 'x \<Rightarrow> 'y spmf) z x;
+    _ :: unit \<leftarrow> assert_spmf((f::'z \<Rightarrow> 'x \<Rightarrow> bool) z x);
+    _ :: unit \<leftarrow> assert_spmf ((A::'y \<Rightarrow> bool) y);
+    return_spmf ((g::'z \<Rightarrow> 'x \<Rightarrow> 'y \<Rightarrow> bool) z x y) }"
+proof -
+  have "\<forall>z x. do {
+    _ :: unit \<leftarrow> assert_spmf((f::'z \<Rightarrow> 'x \<Rightarrow> bool) z x);
+    y::'y \<leftarrow> (Y:: 'z \<Rightarrow> 'x \<Rightarrow> 'y spmf) z x;
+    _ :: unit \<leftarrow> assert_spmf ((A::'y \<Rightarrow> bool) y);
+    return_spmf ((g::'z \<Rightarrow> 'x \<Rightarrow> 'y \<Rightarrow> bool) z x y) }
+  = do {
+    y::'y \<leftarrow> (Y:: 'z \<Rightarrow> 'x \<Rightarrow> 'y spmf) z x;
+    _ :: unit \<leftarrow> assert_spmf((f::'z \<Rightarrow> 'x \<Rightarrow> bool) z x);
+    _ :: unit \<leftarrow> assert_spmf ((A::'y \<Rightarrow> bool) y);
+    return_spmf ((g::'z \<Rightarrow> 'x \<Rightarrow> 'y \<Rightarrow> bool) z x y) }"
+    using bind_commute_spmf by fast
+  then show ?thesis by presburger
+qed
+
+lemma pull_down_assert_spmf_with_assert:
+"do {
+    z::'z \<leftarrow> Z:: 'z spmf;
+    x::'x \<leftarrow> (X:: 'z \<Rightarrow> 'x spmf) z;
+    _ :: unit \<leftarrow> assert_spmf((f::'z \<Rightarrow> 'x \<Rightarrow> bool) z x);
+    y::'y \<leftarrow> (Y:: 'z \<Rightarrow> 'x \<Rightarrow> 'y spmf) z x;
+    _ :: unit \<leftarrow> assert_spmf((g::'z \<Rightarrow> 'x \<Rightarrow> 'y \<Rightarrow> bool) z x y);
+    return_spmf True }
+  = do {
+    z::'z \<leftarrow> Z:: 'z spmf;
+    x::'x \<leftarrow> (X:: 'z \<Rightarrow> 'x spmf) z;
+    y::'y \<leftarrow> (Y:: 'z \<Rightarrow> 'x \<Rightarrow> 'y spmf) z x;
+    _ :: unit \<leftarrow> assert_spmf((f::'z \<Rightarrow> 'x \<Rightarrow> bool) z x);
+    _ :: unit \<leftarrow> assert_spmf((g::'z \<Rightarrow> 'x \<Rightarrow> 'y \<Rightarrow> bool) z x y);
+    return_spmf True }"
+proof -
+  have "\<forall>z x. do {
+    _ :: unit \<leftarrow> assert_spmf((f::'z \<Rightarrow> 'x \<Rightarrow> bool) z x);
+    y::'y \<leftarrow> (Y:: 'z \<Rightarrow> 'x \<Rightarrow> 'y spmf) z x;
+    _ :: unit \<leftarrow> assert_spmf((g::'z \<Rightarrow> 'x \<Rightarrow> 'y \<Rightarrow> bool) z x y);
+    return_spmf True }
+  = do {
+    y::'y \<leftarrow> (Y:: 'z \<Rightarrow> 'x \<Rightarrow> 'y spmf) z x;
+    _ :: unit \<leftarrow> assert_spmf((f::'z \<Rightarrow> 'x \<Rightarrow> bool) z x);
+    _ :: unit \<leftarrow> assert_spmf((g::'z \<Rightarrow> 'x \<Rightarrow> 'y \<Rightarrow> bool) z x y);
+    return_spmf True}"
+    using bind_commute_spmf by fast
+  then show ?thesis by presburger
+qed
+
+lemma key_gen_alt_def: "key_gen = do {
+    x :: nat \<leftarrow> sample_uniform (order G\<^sub>p);
+    let \<alpha>::'e mod_ring = of_int_mod_ring (int x) in
+    return_spmf (map (\<lambda>t. \<^bold>g\<^bsub>G\<^sub>p\<^esub> ^\<^bsub>G\<^sub>p\<^esub> (\<alpha>^t)) [0..<max_deg+1])
+  }"
+  unfolding key_gen_def Setup_def Let_def split_def by simp
+
+declare [[show_types]]
+lemma knowledge_soundness_game_alt_def: 
+  "knowledge_soundness_game E \<A> \<A>' = 
+   TRY do {
+    x :: nat \<leftarrow> sample_uniform (order G\<^sub>p);
+    let \<alpha> = of_int_mod_ring (int x);
+    let PK = map (\<lambda>t. \<^bold>g\<^bsub>G\<^sub>p\<^esub> ^\<^bsub>G\<^sub>p\<^esub> (\<alpha>^t)) [0..<max_deg+1];
+    (C,calc_vec) \<leftarrow> \<A> PK;
+    let \<phi> = E C calc_vec;
+    (i, B, r_x, w_B) \<leftarrow> \<A>' PK C calc_vec;
+    _ :: unit \<leftarrow> assert_spmf (length PK = length calc_vec 
+            \<and> C = fold (\<lambda> i acc. acc \<otimes>\<^bsub>G\<^sub>p\<^esub> PK!i ^\<^bsub>G\<^sub>p\<^esub> (calc_vec!i)) [0..<length PK] \<one>\<^bsub>G\<^sub>p\<^esub>
+            \<and> i \<in> B  
+            \<and> valid_batch_msg r_x w_B B
+            \<and> VerifyEvalBatch PK C B r_x w_B 
+            \<and> poly r_x i \<noteq> poly \<phi> i);
+   return_spmf True
+  } ELSE return_spmf False"
+proof -
+  note [simp] = Let_def split_def
+  have "do {
+  PK \<leftarrow> key_gen;
+  (C,calc_vec) \<leftarrow> \<A> PK;
+  _ :: unit \<leftarrow> assert_spmf (length PK = length calc_vec 
+                          \<and> C = fold (\<lambda> i acc. acc \<otimes>\<^bsub>G\<^sub>p\<^esub> PK!i ^\<^bsub>G\<^sub>p\<^esub> (calc_vec!i)) [0..<length PK] \<one>\<^bsub>G\<^sub>p\<^esub>);  
+  (i, B, r_x, w_B) \<leftarrow> \<A>' PK C calc_vec;
+    _ :: unit \<leftarrow> assert_spmf (i \<in> B  \<and> valid_batch_msg r_x w_B B);
+  return_spmf (VerifyEvalBatch PK C B r_x w_B \<and> poly r_x i \<noteq> poly (E C calc_vec) i)} 
+  = 
+  do {
+  PK \<leftarrow> key_gen;
+  (C,calc_vec) \<leftarrow> \<A> PK;
+  (i, B, r_x, w_B) \<leftarrow> \<A>' PK C calc_vec;
+  _ :: unit \<leftarrow> assert_spmf (length PK = length calc_vec 
+                          \<and> C = fold (\<lambda> i acc. acc \<otimes>\<^bsub>G\<^sub>p\<^esub> PK!i ^\<^bsub>G\<^sub>p\<^esub> (calc_vec!i)) [0..<length PK] \<one>\<^bsub>G\<^sub>p\<^esub>);  
+  _ :: unit \<leftarrow> assert_spmf (i \<in> B  \<and> valid_batch_msg r_x w_B B);  
+  return_spmf (VerifyEvalBatch PK C B r_x w_B \<and> poly r_x i \<noteq> poly (E C calc_vec) i)}"
+    using pull_down_assert_spmf_with_return[of key_gen \<A>] by fastforce
+  then have "knowledge_soundness_game E \<A> \<A>' = 
+  TRY do {
+    PK \<leftarrow> key_gen;
+    (C,calc_vec) \<leftarrow> \<A> PK;
+    let \<phi> = E C calc_vec;
+    (i, B, r_x, w_B) \<leftarrow> \<A>' PK C calc_vec;
+    _ :: unit \<leftarrow> assert_spmf (length PK = length calc_vec 
+                            \<and> C = fold (\<lambda> i acc. acc \<otimes>\<^bsub>G\<^sub>p\<^esub> PK!i ^\<^bsub>G\<^sub>p\<^esub> (calc_vec!i)) [0..<length PK] \<one>\<^bsub>G\<^sub>p\<^esub>);  
+    _ :: unit \<leftarrow> assert_spmf (i \<in> B  \<and> valid_batch_msg r_x w_B B);
+    return_spmf (VerifyEvalBatch PK C B r_x w_B \<and> poly r_x i \<noteq> poly (E C calc_vec) i)
+  } ELSE return_spmf False"
+    unfolding knowledge_soundness_game_def by algebra
+  also have "\<dots> = TRY do {
+    PK \<leftarrow> key_gen;
+    TRY do {
+    (C,calc_vec) \<leftarrow> \<A> PK;
+    TRY do {
+    let \<phi> = E C calc_vec;
+    TRY do {
+    (i, B, r_x, w_B) \<leftarrow> \<A>' PK C calc_vec;
+    TRY do {
+     _ :: unit \<leftarrow> assert_spmf (length PK = length calc_vec 
+                            \<and> C = fold (\<lambda> i acc. acc \<otimes>\<^bsub>G\<^sub>p\<^esub> PK!i ^\<^bsub>G\<^sub>p\<^esub> (calc_vec!i)) [0..<length PK] \<one>\<^bsub>G\<^sub>p\<^esub>);  
+    TRY do {
+    _ :: unit \<leftarrow> assert_spmf (i \<in> B  \<and> valid_batch_msg r_x w_B B);  
+    TRY return_spmf (VerifyEvalBatch PK C B r_x w_B \<and> poly r_x i \<noteq> poly \<phi> i)  ELSE return_spmf False
+    } ELSE return_spmf False
+    } ELSE return_spmf False
+    } ELSE return_spmf False
+    } ELSE return_spmf False
+    } ELSE return_spmf False
+  } ELSE return_spmf False"
+   unfolding split_def Let_def
+   by (fold try_bind_spmf_lossless2[OF lossless_return_spmf])simp
+  also have "\<dots> = TRY do {
+    PK \<leftarrow> key_gen;
+    TRY do {
+    (C,calc_vec) \<leftarrow> \<A> PK;
+    TRY do {
+    let \<phi> = E C calc_vec;
+    TRY do {
+    (i, B, r_x, w_B) \<leftarrow> \<A>' PK C calc_vec;
+    TRY do {
+     _ :: unit \<leftarrow> assert_spmf (length PK = length calc_vec 
+                            \<and> C = fold (\<lambda> i acc. acc \<otimes>\<^bsub>G\<^sub>p\<^esub> PK!i ^\<^bsub>G\<^sub>p\<^esub> (calc_vec!i)) [0..<length PK] \<one>\<^bsub>G\<^sub>p\<^esub>);  
+    TRY do {
+    _ :: unit \<leftarrow> assert_spmf (i \<in> B  \<and> valid_batch_msg r_x w_B B);  
+    _ :: unit \<leftarrow> assert_spmf (VerifyEvalBatch PK C B r_x w_B \<and> poly r_x i \<noteq> poly \<phi> i);
+    return_spmf True
+    } ELSE return_spmf False
+    } ELSE return_spmf False
+    } ELSE return_spmf False
+    } ELSE return_spmf False
+    } ELSE return_spmf False
+  } ELSE return_spmf False"
+   by(auto simp add: try_bind_assert_spmf try_spmf_return_spmf1 intro!: try_spmf_cong bind_spmf_cong)
+  also have "\<dots> = TRY do {
+    PK \<leftarrow> key_gen;
+    TRY do {
+    (C,calc_vec) \<leftarrow> \<A> PK;
+    TRY do {
+    let \<phi> = E C calc_vec;
+    TRY do {
+    (i, B, r_x, w_B) \<leftarrow> \<A>' PK C calc_vec;
+    TRY do {
+     _ :: unit \<leftarrow> assert_spmf (length PK = length calc_vec 
+            \<and> C = fold (\<lambda> i acc. acc \<otimes>\<^bsub>G\<^sub>p\<^esub> PK!i ^\<^bsub>G\<^sub>p\<^esub> (calc_vec!i)) [0..<length PK] \<one>\<^bsub>G\<^sub>p\<^esub>);  
+    TRY do {
+    _ :: unit \<leftarrow> assert_spmf (i \<in> B  \<and> valid_batch_msg r_x w_B B
+            \<and> VerifyEvalBatch PK C B r_x w_B \<and> poly r_x i \<noteq> poly \<phi> i);
+    return_spmf True
+    } ELSE return_spmf False
+    } ELSE return_spmf False
+    } ELSE return_spmf False
+    } ELSE return_spmf False
+    } ELSE return_spmf False
+  } ELSE return_spmf False"
+    using assert_anding by presburger
+   also have "\<dots> = TRY do {
+    PK \<leftarrow> key_gen;
+    TRY do {
+    (C,calc_vec) \<leftarrow> \<A> PK;
+    TRY do {
+    let \<phi> = E C calc_vec;
+    TRY do {
+    (i, B, r_x, w_B) \<leftarrow> \<A>' PK C calc_vec;
+    TRY do {
+     _ :: unit \<leftarrow> assert_spmf (length PK = length calc_vec 
+            \<and> C = fold (\<lambda> i acc. acc \<otimes>\<^bsub>G\<^sub>p\<^esub> PK!i ^\<^bsub>G\<^sub>p\<^esub> (calc_vec!i)) [0..<length PK] \<one>\<^bsub>G\<^sub>p\<^esub>);
+    _ :: unit \<leftarrow> assert_spmf (i \<in> B  \<and> valid_batch_msg r_x w_B B
+            \<and> VerifyEvalBatch PK C B r_x w_B \<and> poly r_x i \<noteq> poly \<phi> i);
+    return_spmf True
+    } ELSE return_spmf False
+    } ELSE return_spmf False
+    } ELSE return_spmf False
+    } ELSE return_spmf False
+  } ELSE return_spmf False"
+    unfolding split_def Let_def
+    by(fold try_bind_spmf_lossless2[OF lossless_return_spmf]) simp
+   also have "\<dots> = TRY do {
+    PK \<leftarrow> key_gen;
+    TRY do {
+    (C,calc_vec) \<leftarrow> \<A> PK;
+    TRY do {
+    let \<phi> = E C calc_vec;
+    TRY do {
+    (i, B, r_x, w_B) \<leftarrow> \<A>' PK C calc_vec;
+    TRY do {
+     _ :: unit \<leftarrow> assert_spmf (length PK = length calc_vec 
+            \<and> C = fold (\<lambda> i acc. acc \<otimes>\<^bsub>G\<^sub>p\<^esub> PK!i ^\<^bsub>G\<^sub>p\<^esub> (calc_vec!i)) [0..<length PK] \<one>\<^bsub>G\<^sub>p\<^esub>
+            \<and> i \<in> B  \<and> valid_batch_msg r_x w_B B
+            \<and> VerifyEvalBatch PK C B r_x w_B \<and> poly r_x i \<noteq> poly \<phi> i);
+    return_spmf True
+    } ELSE return_spmf False
+    } ELSE return_spmf False
+    } ELSE return_spmf False
+    } ELSE return_spmf False
+  } ELSE return_spmf False"
+     using assert_anding by presburger
+   text \<open>next step, add assert PK construction\<close>
+  also have "\<dots> = TRY do {
+    PK \<leftarrow> key_gen;
+    (C,calc_vec) \<leftarrow> \<A> PK;
+    let \<phi> = E C calc_vec;
+    (i, B, r_x, w_B) \<leftarrow> \<A>' PK C calc_vec;
+     _ :: unit \<leftarrow> assert_spmf (length PK = length calc_vec 
+            \<and> C = fold (\<lambda> i acc. acc \<otimes>\<^bsub>G\<^sub>p\<^esub> PK!i ^\<^bsub>G\<^sub>p\<^esub> (calc_vec!i)) [0..<length PK] \<one>\<^bsub>G\<^sub>p\<^esub>
+            \<and> i \<in> B  \<and> valid_batch_msg r_x w_B B
+            \<and> VerifyEvalBatch PK C B r_x w_B \<and> poly r_x i \<noteq> poly \<phi> i);
+    return_spmf True
+  } ELSE return_spmf False"
+    unfolding split_def Let_def
+    by(fold try_bind_spmf_lossless2[OF lossless_return_spmf]) simp
+  also have "\<dots> = TRY do {
+    x :: nat \<leftarrow> sample_uniform (order G\<^sub>p);
+    let \<alpha> = of_int_mod_ring (int x);
+    PK \<leftarrow> return_spmf (map (\<lambda>t. \<^bold>g\<^bsub>G\<^sub>p\<^esub> ^\<^bsub>G\<^sub>p\<^esub> (\<alpha>^t)) [0..<max_deg+1]);
+    (C,calc_vec) \<leftarrow> \<A> PK;
+    let \<phi> = E C calc_vec;
+    (i, B, r_x, w_B) \<leftarrow> \<A>' PK C calc_vec;
+     _ :: unit \<leftarrow> assert_spmf (length PK = length calc_vec 
+            \<and> C = fold (\<lambda> i acc. acc \<otimes>\<^bsub>G\<^sub>p\<^esub> PK!i ^\<^bsub>G\<^sub>p\<^esub> (calc_vec!i)) [0..<length PK] \<one>\<^bsub>G\<^sub>p\<^esub>
+            \<and> i \<in> B  \<and> valid_batch_msg r_x w_B B
+            \<and> VerifyEvalBatch PK C B r_x w_B \<and> poly r_x i \<noteq> poly \<phi> i);
+    return_spmf True
+  } ELSE return_spmf False"
+     using key_gen_alt_def
+     by (smt (verit, ccfv_SIG) bind_spmf_assoc bind_spmf_cong)
+    also have "\<dots> = TRY do {
+    x :: nat \<leftarrow> sample_uniform (order G\<^sub>p);
+    let \<alpha> = of_int_mod_ring (int x);
+    let PK = map (\<lambda>t. \<^bold>g\<^bsub>G\<^sub>p\<^esub> ^\<^bsub>G\<^sub>p\<^esub> (\<alpha>^t)) [0..<max_deg+1];
+    (C,calc_vec) \<leftarrow> \<A> PK;
+    let \<phi> = E C calc_vec;
+    (i, B, r_x, w_B) \<leftarrow> \<A>' PK C calc_vec;
+     _ :: unit \<leftarrow> assert_spmf (length PK = length calc_vec 
+            \<and> C = fold (\<lambda> i acc. acc \<otimes>\<^bsub>G\<^sub>p\<^esub> PK!i ^\<^bsub>G\<^sub>p\<^esub> (calc_vec!i)) [0..<length PK] \<one>\<^bsub>G\<^sub>p\<^esub>
+            \<and> i \<in> B  \<and> valid_batch_msg r_x w_B B
+            \<and> VerifyEvalBatch PK C B r_x w_B \<and> poly r_x i \<noteq> poly \<phi> i);
+    return_spmf True
+  } ELSE return_spmf False"
+      using return_bind_spmf by meson
+  finally show ?thesis .
+qed
+
+lemma bind_game_knowledge_soundness_reduction_alt_def: 
+  "bind_game (knowledge_soundness_reduction E \<A> \<A>') = 
+  TRY do {
+    x :: nat \<leftarrow> sample_uniform (order G\<^sub>p);
+    let \<alpha> = of_int_mod_ring (int x);
+    let PK = map (\<lambda>t. \<^bold>g\<^bsub>G\<^sub>p\<^esub> ^\<^bsub>G\<^sub>p\<^esub> (\<alpha>^t)) [0..<max_deg+1];
+    (C,calc_vec) \<leftarrow> \<A> PK;
+    let \<phi> = E C calc_vec;
+    (i, B, r_x, w_B) \<leftarrow> \<A>' PK C calc_vec;
+    _ :: unit \<leftarrow> assert_spmf (length PK = length calc_vec
+            \<and> C = fold (\<lambda> i acc. acc \<otimes>\<^bsub>G\<^sub>p\<^esub> PK!i ^\<^bsub>G\<^sub>p\<^esub> (calc_vec!i)) [0..<length PK] \<one>\<^bsub>G\<^sub>p\<^esub>
+            \<and> i \<in> B 
+            \<and> poly \<phi> i \<noteq>  poly r_x i
+            \<and> valid_msg (poly \<phi> i) (createWitness PK \<phi> i)
+            \<and> valid_batch_msg r_x w_B B
+            \<and> VerifyEval PK C i (poly \<phi> i) (createWitness PK \<phi> i) 
+            \<and> VerifyEvalBatch PK C B r_x w_B);
+       return_spmf True
+    } ELSE return_spmf False"
+proof -
+  have "bind_game (knowledge_soundness_reduction E \<A> \<A>') = TRY do {
+  PK \<leftarrow> key_gen;
+  (C, i, \<phi>_i, w_i, B, w_B, r_x) \<leftarrow> (knowledge_soundness_reduction E \<A> \<A>') PK;
+  _ :: unit \<leftarrow> assert_spmf (i \<in> B \<and> \<phi>_i \<noteq> poly r_x i \<and> valid_msg \<phi>_i w_i \<and> valid_batch_msg r_x w_B B); 
+  let b = VerifyEval PK C i \<phi>_i w_i;
+  let b' = VerifyEvalBatch PK C B r_x w_B;
+  _::unit \<leftarrow> assert_spmf (b \<and> b');
+  return_spmf True} ELSE return_spmf False" 
+    by (fact bind_game_alt_def)
+  also have "\<dots> = TRY do {
+  PK \<leftarrow> key_gen;
+  (C,calc_vec) \<leftarrow> \<A> PK;
+  _ :: unit \<leftarrow> assert_spmf (length PK = length calc_vec 
+                          \<and> C = fold (\<lambda> i acc. acc \<otimes>\<^bsub>G\<^sub>p\<^esub> PK!i ^\<^bsub>G\<^sub>p\<^esub> (calc_vec!i)) [0..<length PK] \<one>\<^bsub>G\<^sub>p\<^esub>);  
+  let \<phi> = E C calc_vec;
+  (i, B, r_x, w_B) \<leftarrow> \<A>' PK C calc_vec;
+  let \<phi>_i = poly \<phi> i;
+  let w_i = createWitness PK \<phi> i;
+  _ :: unit \<leftarrow> assert_spmf (i \<in> B \<and> \<phi>_i \<noteq> poly r_x i \<and> valid_msg \<phi>_i w_i \<and> valid_batch_msg r_x w_B B); 
+  let b = VerifyEval PK C i \<phi>_i w_i;
+  let b' = VerifyEvalBatch PK C B r_x w_B;
+  _::unit \<leftarrow> assert_spmf (b \<and> b');
+  return_spmf True} ELSE return_spmf False"
+  unfolding knowledge_soundness_reduction_def by (simp add: split_def Let_def)
+  also have "\<dots> = TRY do {
+    PK \<leftarrow> key_gen;
+    TRY do{
+    (C,calc_vec) \<leftarrow> \<A> PK;
+    TRY do {
+    _ :: unit \<leftarrow> assert_spmf (length PK = length calc_vec 
+                            \<and> C = fold (\<lambda> i acc. acc \<otimes>\<^bsub>G\<^sub>p\<^esub> PK!i ^\<^bsub>G\<^sub>p\<^esub> (calc_vec!i)) [0..<length PK] \<one>\<^bsub>G\<^sub>p\<^esub>);  
+    let \<phi> = E C calc_vec;
+    TRY do {
+    (i, B, r_x, w_B) \<leftarrow> \<A>' PK C calc_vec;
+    let \<phi>_i = poly \<phi> i;
+    let w_i = createWitness PK \<phi> i;
+    TRY do {
+    _ :: unit \<leftarrow> assert_spmf (i \<in> B \<and> \<phi>_i \<noteq> poly r_x i \<and> valid_msg \<phi>_i w_i \<and> valid_batch_msg r_x w_B B); 
+    let b = VerifyEval PK C i \<phi>_i w_i;
+    let b' = VerifyEvalBatch PK C B r_x w_B;
+    _::unit \<leftarrow> assert_spmf (b \<and> b');
+    return_spmf True
+    } ELSE return_spmf False 
+    } ELSE return_spmf False 
+    } ELSE return_spmf False 
+    } ELSE return_spmf False 
+  } ELSE return_spmf False"
+   unfolding split_def Let_def 
+   by(fold try_bind_spmf_lossless2[OF lossless_return_spmf]) simp
+  also have "\<dots> = TRY do {
+    PK \<leftarrow> key_gen;
+    TRY do{
+    (C,calc_vec) \<leftarrow> \<A> PK;
+    TRY do {
+    _ :: unit \<leftarrow> assert_spmf (length PK = length calc_vec 
+                            \<and> C = fold (\<lambda> i acc. acc \<otimes>\<^bsub>G\<^sub>p\<^esub> PK!i ^\<^bsub>G\<^sub>p\<^esub> (calc_vec!i)) [0..<length PK] \<one>\<^bsub>G\<^sub>p\<^esub>);  
+    let \<phi> = E C calc_vec;
+    TRY do {
+    (i, B, r_x, w_B) \<leftarrow> \<A>' PK C calc_vec;
+    let \<phi>_i = poly \<phi> i;
+    let w_i = createWitness PK \<phi> i;
+    TRY do {
+    _ :: unit \<leftarrow> assert_spmf (i \<in> B \<and> \<phi>_i \<noteq> poly r_x i 
+                            \<and> valid_msg \<phi>_i w_i \<and> valid_batch_msg r_x w_B B
+                            \<and> VerifyEval PK C i \<phi>_i w_i \<and> VerifyEvalBatch PK C B r_x w_B);
+    return_spmf True
+    } ELSE return_spmf False 
+    } ELSE return_spmf False 
+    } ELSE return_spmf False 
+    } ELSE return_spmf False 
+  } ELSE return_spmf False"
+    using assert_anding by presburger
+  also have "\<dots> = TRY do {
+    PK \<leftarrow> key_gen;
+    (C,calc_vec) \<leftarrow> \<A> PK;
+    _ :: unit \<leftarrow> assert_spmf (length PK = length calc_vec 
+                            \<and> C = fold (\<lambda> i acc. acc \<otimes>\<^bsub>G\<^sub>p\<^esub> PK!i ^\<^bsub>G\<^sub>p\<^esub> (calc_vec!i)) [0..<length PK] \<one>\<^bsub>G\<^sub>p\<^esub>);  
+    let \<phi> = E C calc_vec;
+    (i, B, r_x, w_B) \<leftarrow> \<A>' PK C calc_vec;
+    let \<phi>_i = poly \<phi> i;
+    let w_i = createWitness PK \<phi> i;
+    _ :: unit \<leftarrow> assert_spmf (i \<in> B \<and> \<phi>_i \<noteq> poly r_x i 
+                            \<and> valid_msg \<phi>_i w_i \<and> valid_batch_msg r_x w_B B
+                            \<and> VerifyEval PK C i \<phi>_i w_i \<and> VerifyEvalBatch PK C B r_x w_B);
+    return_spmf True
+  } ELSE return_spmf False"
+   unfolding split_def Let_def 
+   by(fold try_bind_spmf_lossless2[OF lossless_return_spmf]) simp
+  also have "\<dots> = TRY do {
+    PK \<leftarrow> key_gen;
+    (C,calc_vec) \<leftarrow> \<A> PK;
+    
+    (i, B, r_x, w_B) \<leftarrow> \<A>' PK C calc_vec;
+    _ :: unit \<leftarrow> assert_spmf (length PK = length calc_vec 
+                            \<and> C = fold (\<lambda> i acc. acc \<otimes>\<^bsub>G\<^sub>p\<^esub> PK!i ^\<^bsub>G\<^sub>p\<^esub> (calc_vec!i)) [0..<length PK] \<one>\<^bsub>G\<^sub>p\<^esub>);  
+    let \<phi> = E C calc_vec;
+    let \<phi>_i = poly \<phi> i;
+    let w_i = createWitness PK \<phi> i;
+    _ :: unit \<leftarrow> assert_spmf (i \<in> B \<and> \<phi>_i \<noteq> poly r_x i 
+                            \<and> valid_msg \<phi>_i w_i \<and> valid_batch_msg r_x w_B B
+                            \<and> VerifyEval PK C i \<phi>_i w_i \<and> VerifyEvalBatch PK C B r_x w_B);
+    return_spmf True
+  } ELSE return_spmf False"
+  proof -
+    have "do {
+    PK \<leftarrow> key_gen;
+    (C,calc_vec) \<leftarrow> \<A> PK;
+    _ :: unit \<leftarrow> assert_spmf (length PK = length calc_vec 
+                            \<and> C = fold (\<lambda> i acc. acc \<otimes>\<^bsub>G\<^sub>p\<^esub> PK!i ^\<^bsub>G\<^sub>p\<^esub> (calc_vec!i)) [0..<length PK] \<one>\<^bsub>G\<^sub>p\<^esub>);  
+    let \<phi> = E C calc_vec;
+    (i, B, r_x, w_B) \<leftarrow> \<A>' PK C calc_vec;
+    let \<phi>_i = poly \<phi> i;
+    let w_i = createWitness PK \<phi> i;
+    _ :: unit \<leftarrow> assert_spmf (i \<in> B \<and> \<phi>_i \<noteq> poly r_x i 
+                            \<and> valid_msg \<phi>_i w_i \<and> valid_batch_msg r_x w_B B
+                            \<and> VerifyEval PK C i \<phi>_i w_i \<and> VerifyEvalBatch PK C B r_x w_B);
+    return_spmf True
+    } = do {
+    PK \<leftarrow> key_gen;
+    (C,calc_vec) \<leftarrow> \<A> PK;
+    
+    (i, B, r_x, w_B) \<leftarrow> \<A>' PK C calc_vec;
+    _ :: unit \<leftarrow> assert_spmf (length PK = length calc_vec 
+                            \<and> C = fold (\<lambda> i acc. acc \<otimes>\<^bsub>G\<^sub>p\<^esub> PK!i ^\<^bsub>G\<^sub>p\<^esub> (calc_vec!i)) [0..<length PK] \<one>\<^bsub>G\<^sub>p\<^esub>);  
+    let \<phi> = E C calc_vec;
+    let \<phi>_i = poly \<phi> i;
+    let w_i = createWitness PK \<phi> i;
+    _ :: unit \<leftarrow> assert_spmf (i \<in> B \<and> \<phi>_i \<noteq> poly r_x i 
+                            \<and> valid_msg \<phi>_i w_i \<and> valid_batch_msg r_x w_B B
+                            \<and> VerifyEval PK C i \<phi>_i w_i \<and> VerifyEvalBatch PK C B r_x w_B);
+    return_spmf True
+    }"
+      using pull_down_assert_spmf_with_assert[of key_gen \<A>] 
+      by (simp add: Let_def split_def)
+    then show ?thesis by argo
+  qed
+  also have "\<dots> = TRY do {
+    PK \<leftarrow> key_gen;
+    TRY do {
+    (C,calc_vec) \<leftarrow> \<A> PK;
+    TRY do {
+    (i, B, r_x, w_B) \<leftarrow> \<A>' PK C calc_vec;
+    TRY do {
+    _ :: unit \<leftarrow> assert_spmf (length PK = length calc_vec 
+                            \<and> C = fold (\<lambda> i acc. acc \<otimes>\<^bsub>G\<^sub>p\<^esub> PK!i ^\<^bsub>G\<^sub>p\<^esub> (calc_vec!i)) [0..<length PK] \<one>\<^bsub>G\<^sub>p\<^esub>);  
+    let \<phi> = E C calc_vec;
+    let \<phi>_i = poly \<phi> i;
+    let w_i = createWitness PK \<phi> i;
+    _ :: unit \<leftarrow> assert_spmf (i \<in> B \<and> \<phi>_i \<noteq> poly r_x i 
+                            \<and> valid_msg \<phi>_i w_i \<and> valid_batch_msg r_x w_B B
+                            \<and> VerifyEval PK C i \<phi>_i w_i \<and> VerifyEvalBatch PK C B r_x w_B);
+    return_spmf True
+    } ELSE return_spmf False
+    } ELSE return_spmf False 
+    } ELSE return_spmf False
+  } ELSE return_spmf False"
+  unfolding split_def Let_def 
+  by(fold try_bind_spmf_lossless2[OF lossless_return_spmf]) simp
+  also have "\<dots> = TRY do {
+    PK \<leftarrow> key_gen;
+    TRY do {
+    (C,calc_vec) \<leftarrow> \<A> PK;
+    TRY do {
+    (i, B, r_x, w_B) \<leftarrow> \<A>' PK C calc_vec;
+    TRY do {
+    let \<phi> = E C calc_vec;
+    let \<phi>_i = poly \<phi> i;
+    let w_i = createWitness PK \<phi> i;
+    _ :: unit \<leftarrow> assert_spmf (length PK = length calc_vec 
+                            \<and> C = fold (\<lambda> i acc. acc \<otimes>\<^bsub>G\<^sub>p\<^esub> PK!i ^\<^bsub>G\<^sub>p\<^esub> (calc_vec!i)) [0..<length PK] \<one>\<^bsub>G\<^sub>p\<^esub>
+                            \<and> i \<in> B \<and> \<phi>_i \<noteq> poly r_x i 
+                            \<and> valid_msg \<phi>_i w_i \<and> valid_batch_msg r_x w_B B
+                            \<and> VerifyEval PK C i \<phi>_i w_i \<and> VerifyEvalBatch PK C B r_x w_B);
+    return_spmf True
+    } ELSE return_spmf False
+    } ELSE return_spmf False 
+    } ELSE return_spmf False
+  } ELSE return_spmf False"
+    unfolding Let_def
+    using assert_anding by presburger
+  also have "\<dots> = TRY do {
+    PK \<leftarrow> key_gen;
+    (C,calc_vec) \<leftarrow> \<A> PK;
+    (i, B, r_x, w_B) \<leftarrow> \<A>' PK C calc_vec;
+    let \<phi> = E C calc_vec;
+    let \<phi>_i = poly \<phi> i;
+    let w_i = createWitness PK \<phi> i;
+    _ :: unit \<leftarrow> assert_spmf (length PK = length calc_vec 
+                            \<and> C = fold (\<lambda> i acc. acc \<otimes>\<^bsub>G\<^sub>p\<^esub> PK!i ^\<^bsub>G\<^sub>p\<^esub> (calc_vec!i)) [0..<length PK] \<one>\<^bsub>G\<^sub>p\<^esub>
+                            \<and> i \<in> B \<and> \<phi>_i \<noteq> poly r_x i 
+                            \<and> valid_msg \<phi>_i w_i \<and> valid_batch_msg r_x w_B B
+                            \<and> VerifyEval PK C i \<phi>_i w_i \<and> VerifyEvalBatch PK C B r_x w_B);
+    return_spmf True
+  } ELSE return_spmf False"
+   unfolding split_def Let_def 
+   by(fold try_bind_spmf_lossless2[OF lossless_return_spmf]) simp
+ text \<open>make PK definition extractable\<close>
+  also have "\<dots> = TRY do {
+    x :: nat \<leftarrow> sample_uniform (order G\<^sub>p);
+    let \<alpha> = of_int_mod_ring (int x);
+    PK \<leftarrow> return_spmf (map (\<lambda>t. \<^bold>g\<^bsub>G\<^sub>p\<^esub> ^\<^bsub>G\<^sub>p\<^esub> (\<alpha>^t)) [0..<max_deg+1]);
+    (C,calc_vec) \<leftarrow> \<A> PK;
+    (i, B, r_x, w_B) \<leftarrow> \<A>' PK C calc_vec;
+    let \<phi> = E C calc_vec;
+    let \<phi>_i = poly \<phi> i;
+    let w_i = createWitness PK \<phi> i;
+    _ :: unit \<leftarrow> assert_spmf (length PK = length calc_vec 
+                            \<and> C = fold (\<lambda> i acc. acc \<otimes>\<^bsub>G\<^sub>p\<^esub> PK!i ^\<^bsub>G\<^sub>p\<^esub> (calc_vec!i)) [0..<length PK] \<one>\<^bsub>G\<^sub>p\<^esub>
+                            \<and> i \<in> B \<and> \<phi>_i \<noteq> poly r_x i 
+                            \<and> valid_msg \<phi>_i w_i \<and> valid_batch_msg r_x w_B B
+                            \<and> VerifyEval PK C i \<phi>_i w_i \<and> VerifyEvalBatch PK C B r_x w_B);
+       return_spmf True
+    } ELSE return_spmf False"
+    using key_gen_alt_def
+    by (smt (verit, ccfv_SIG) bind_spmf_assoc bind_spmf_cong)
+  also have "\<dots> = TRY do {
+    x :: nat \<leftarrow> sample_uniform (order G\<^sub>p);
+    let \<alpha> = of_int_mod_ring (int x);
+    let PK = map (\<lambda>t. \<^bold>g\<^bsub>G\<^sub>p\<^esub> ^\<^bsub>G\<^sub>p\<^esub> (\<alpha>^t)) [0..<max_deg+1];
+    (C,calc_vec) \<leftarrow> \<A> PK;
+    (i, B, r_x, w_B) \<leftarrow> \<A>' PK C calc_vec;
+    let \<phi> = E C calc_vec;
+    let \<phi>_i = poly \<phi> i;
+    let w_i = createWitness PK \<phi> i;
+    _ :: unit \<leftarrow> assert_spmf (length PK = length calc_vec 
+                            \<and> C = fold (\<lambda> i acc. acc \<otimes>\<^bsub>G\<^sub>p\<^esub> PK!i ^\<^bsub>G\<^sub>p\<^esub> (calc_vec!i)) [0..<length PK] \<one>\<^bsub>G\<^sub>p\<^esub>
+                            \<and> i \<in> B \<and> \<phi>_i \<noteq> poly r_x i 
+                            \<and> valid_msg \<phi>_i w_i \<and> valid_batch_msg r_x w_B B
+                            \<and> VerifyEval PK C i \<phi>_i w_i \<and> VerifyEvalBatch PK C B r_x w_B);
+       return_spmf True
+    } ELSE return_spmf False"
+    using return_bind_spmf by meson
+  finally show ?thesis unfolding Let_def .
+qed
+
+lemma asserts_are_equal: 
+  "length (map (\<lambda>t::nat. \<^bold>g ^\<^bsub>G\<^sub>p\<^esub> \<alpha> ^ t) [0::nat..<max_deg + (1::nat)]) = length calc_vec \<and>
+                      C =
+                      fold
+                       (\<lambda>(i::nat) acc::'a.
+                           acc \<otimes>\<^bsub>G\<^sub>p\<^esub> map (\<lambda>t::nat. \<^bold>g ^\<^bsub>G\<^sub>p\<^esub> \<alpha> ^ t) [0::nat..<max_deg + (1::nat)] ! i ^\<^bsub>G\<^sub>p\<^esub> calc_vec ! i)
+                       [0::nat..<length (map (\<lambda>t::nat. \<^bold>g ^\<^bsub>G\<^sub>p\<^esub> \<alpha> ^ t) [0::nat..<max_deg + (1::nat)])] \<one> \<and>
+                      i \<in> B \<and>
+                      valid_batch_msg r_x w_B B \<and>
+                      VerifyEvalBatch (map (\<lambda>t::nat. \<^bold>g ^\<^bsub>G\<^sub>p\<^esub> \<alpha> ^ t) [0::nat..<max_deg + (1::nat)]) C B r_x w_B \<and>
+                      poly r_x i \<noteq> poly (E C calc_vec) i 
+      \<longleftrightarrow> 
+  length (map (\<lambda>t::nat. \<^bold>g ^\<^bsub>G\<^sub>p\<^esub> \<alpha> ^ t) [0::nat..<max_deg + (1::nat)]) = length calc_vec \<and>
+                      C =
+                      fold
+                       (\<lambda>(i::nat) acc::'a.
+                           acc \<otimes>\<^bsub>G\<^sub>p\<^esub> map (\<lambda>t::nat. \<^bold>g ^\<^bsub>G\<^sub>p\<^esub> \<alpha> ^ t) [0::nat..<max_deg + (1::nat)] ! i ^\<^bsub>G\<^sub>p\<^esub> calc_vec ! i)
+                       [0::nat..<length (map (\<lambda>t::nat. \<^bold>g ^\<^bsub>G\<^sub>p\<^esub> \<alpha> ^ t) [0::nat..<max_deg + (1::nat)])] \<one> \<and>
+                      i \<in> B \<and>
+                      poly (E C calc_vec) i \<noteq> poly r_x i \<and>
+                      valid_msg (poly (E C calc_vec) i)
+                       (createWitness (map (\<lambda>t::nat. \<^bold>g ^\<^bsub>G\<^sub>p\<^esub> \<alpha> ^ t) [0::nat..<max_deg + (1::nat)]) (E C calc_vec) i) \<and>
+                      valid_batch_msg r_x w_B B \<and>
+                      VerifyEval (map (\<lambda>t::nat. \<^bold>g ^\<^bsub>G\<^sub>p\<^esub> \<alpha> ^ t) [0::nat..<max_deg + (1::nat)]) C i
+                       (poly (E C calc_vec) i)
+                       (createWitness (map (\<lambda>t::nat. \<^bold>g ^\<^bsub>G\<^sub>p\<^esub> \<alpha> ^ t) [0::nat..<max_deg + (1::nat)]) (E C calc_vec) i) \<and>
+                      VerifyEvalBatch (map (\<lambda>t::nat. \<^bold>g ^\<^bsub>G\<^sub>p\<^esub> \<alpha> ^ t) [0::nat..<max_deg + (1::nat)]) C B r_x w_B"
+  (is "?lhs \<longleftrightarrow> ?rhs")
+proof 
+  assume asm: ?lhs
+  show ?rhs
+  proof (intro conjI)
+    show "length (map (\<lambda>t::nat. \<^bold>g ^ \<alpha> ^ t) [0::nat..<max_deg + (1::nat)]) = length calc_vec"
+      using asm by blast
+    show C: "C =
+    fold (\<lambda>(i::nat) acc::'a. acc \<otimes> map (\<lambda>t::nat. \<^bold>g ^ \<alpha> ^ t) [0::nat..<max_deg + (1::nat)] ! i ^ calc_vec ! i)
+     [0::nat..<length (map (\<lambda>t::nat. \<^bold>g ^ \<alpha> ^ t) [0::nat..<max_deg + (1::nat)])] \<one>"
+      using asm by fast
+    show " i \<in> B"
+      using asm by blast
+    show "poly (E C calc_vec) i \<noteq> poly r_x i"
+      using asm by argo
+    show "valid_msg (poly (E C calc_vec) i)
+     (createWitness (map (\<lambda>t::nat. \<^bold>g ^ \<alpha> ^ t) [0::nat..<max_deg + (1::nat)]) (E C calc_vec) i)"
+      unfolding valid_msg_def createWitness.simps Let_def  sorry
+    show "valid_batch_msg r_x w_B B"
+      using asm by fast
+    show "VerifyEval (map (\<lambda>t::nat. \<^bold>g ^ \<alpha> ^ t) [0::nat..<max_deg + (1::nat)]) C i (poly (E C calc_vec) i)
+     (createWitness (map (\<lambda>t::nat. \<^bold>g ^ \<alpha> ^ t) [0::nat..<max_deg + (1::nat)]) (E C calc_vec) i)"
+      unfolding VerifyEval_def createWitness.simps Let_def C sorry
+    show "VerifyEvalBatch (map (\<lambda>t::nat. \<^bold>g ^ \<alpha> ^ t) [0::nat..<max_deg + (1::nat)]) C B r_x w_B"
+      using asm by linarith
+  qed 
+qed argo
+
+theorem knowledge_soundness_game_eq_bind_game_knowledge_soundness_reduction: 
+  "knowledge_soundness_game E \<A> \<A>' = bind_game (knowledge_soundness_reduction E \<A> \<A>')"
+  unfolding knowledge_soundness_game_alt_def 
+            bind_game_knowledge_soundness_reduction_alt_def
+            Let_def
+  using asserts_are_equal by simp
+
+theorem evaluation_knowledge_soundness: 
+  "knowledge_soundness_game_advantage E \<A> \<A>' 
+  = t_BSDH.advantage (bind_reduction (knowledge_soundness_reduction E \<A> \<A>'))"
+  using knowledge_soundness_game_eq_bind_game_knowledge_soundness_reduction 
+        batchOpening_binding
+  unfolding bind_advantage_def knowledge_soundness_game_advantage_def
+  by algebra
+  
+
+end
